end of day 13/01/19

michael_formal/theory_cleaner.py
@@ -1,7 +1,7 @@
 #!/usr/bin/env python3
 # -*- coding: utf-8 -*-
 """
-Created on Sun Jan 13 11:39:13 2019
+Created on Sun Jan 13 14:20:44 2019
 
 @author: michael
 """
@@ -10,41 +10,42 @@ import re
 import os
 
 root = '/home/michael/Documents/elixir/athena2/michael_formal/'
-lemma_re = re.compile('\s*(have|lemma) ((\w)*?):')
-apply_re = re.compile('\s*(apply|by) \((simp|metis|simp_all) (add|only): ((\w| )*)\s*\)\s*')
-using_re = re.compile('\s*using ((\w| )*)\s*')
-lemmas_re = re.compile('\s*lemmas \w* = ((\w| )*)')
 
 for root, dirs, files in os.walk(root):
     for file in files:
-        if file.endswith("DM_Inference.thy"):
+        if file.endswith(".thy"):
             lemmas_named = set()
             lemmas_used = set()
+            duplicate_names = set()
             filepath = os.path.join(root, file)
-            print(file)
             with open(filepath) as f:
-                for line in f:
-                    named_lemma = lemma_re.match(line)
-                    simps = apply_re.match(line)
-                    using = using_re.match(line)
-                    lemmas = lemmas_re.match(line)
-                    if named_lemma:
-                        lemmas_named.add(named_lemma.group(2))
-#                        print(named_lemma.group(1))
-                    if simps:
-#                        print(simps.group(4).split(' '))
-                        lemmas_used = lemmas_used.union(set(simps.group(4).split(' ')))
-                    if using:
-#                        print(using.group(1).split(' '))
-                        lemmas_used = lemmas_used.union(set(using.group(1).split(' ')))
-                    if lemmas:
-#                        print(lemmas.group(1).split(' '))
-                        lemmas_used = lemmas_used.union(set(lemmas.group(1).split(' ')))
+                theory = f.read()
+                named_lemmas = re.finditer('\s*(have|lemma) ((\w)*?):', theory)
+                applies = re.finditer('\s*(apply|by) \((simp|metis|simp_all) (add|only): ((\w|\.|\s*)*)\s*\)\s*', theory)
+                usings = re.finditer('\s*using ((\w| )*)\s*', theory)
+                lemmas = re.finditer('\s*lemmas \w* = ((\w| )*)', theory)
+            for lemma in named_lemmas:
+#                print(lemma.group(2))
+                if lemma.group(2) in lemmas_named:
+                    duplicate_names.add(lemma.group(2))
+                else:
+                    lemmas_named.add(lemma.group(2))
+            for apply in applies:
+#                print(apply.group(4).split(' '))
+                lemmas_used = lemmas_used.union(set([x.strip() for x in apply.group(4).split(' ')]))
+            for using in usings:
+#                print(using.group(1).split(' '))
+                lemmas_used = lemmas_used.union(set([x.strip() for x in using.group(1).split(' ')]))
+            for lemma in lemmas:
+#                print(lemma.group(1).split(' '))
+                lemmas_used = lemmas_used.union([x.strip() for x in set(lemma.group(1).split(' '))])
 
-            print()
-            print(len(lemmas_named), sorted(list(lemmas_named)))
-            print()
-            print(len(lemmas_used.intersection(lemmas_named)), sorted(list(lemmas_used.intersection(lemmas_named))))
-            print()
-            print(len(lemmas_named.difference(lemmas_used)), sorted(list(lemmas_named.difference(lemmas_used))))
-            print('\n')
+            if len(lemmas_named.difference(lemmas_used)) > 0 or len(duplicate_names) > 0:
+                print(file)
+    #            print(len(lemmas_named), sorted(list(lemmas_named)))
+    #            print()
+    #            print(len(lemmas_used.intersection(lemmas_named)), sorted(list(lemmas_used.intersection(lemmas_named))))
+    #            print()
+                print(len(lemmas_named.difference(lemmas_used)), sorted(list(lemmas_named.difference(lemmas_used))))
+                print(sorted(list(duplicate_names)))
+                print('\n')
