michael_formal/inference/Learn_EFSM.thy
@@ -1,8 +1,813 @@
 theory Learn_EFSM
-  imports Inference SelectionStrategies "../examples/Drinks_Machine" Learn_EFSM_Transitions EFSM_Dot
+  imports Inference SelectionStrategies EFSM_Dot
 begin
 
 declare One_nat_def [simp del]
+
+definition selectCoke :: transition where
+  "selectCoke = \<lparr>Label = ''select'', Arity = 1, Guard = [gexp.Eq (V (I 1)) (L (Str ''coke''))], Outputs = [], Updates = []\<rparr>"
+
+definition coin50_50 :: transition where
+  "coin50_50 = \<lparr>Label = ''coin'', Arity = 1, Guard = [gexp.Eq (V (I 1)) (L (Num 50))], Outputs = [L (Num 50)], Updates = []\<rparr>"
+
+definition coin50_100 :: transition where
+  "coin50_100 = \<lparr>Label = ''coin'', Arity = 1, Guard = [gexp.Eq (V (I 1)) (L (Num 50))], Outputs = [L (Num 100)], Updates = []\<rparr>"
+
+definition vend_coke :: transition where
+  "vend_coke = \<lparr>Label = ''vend'', Arity = 0, Guard = [], Outputs = [L (Str ''coke'')], Updates = []\<rparr>"
+
+definition coin100_100 :: transition where
+  "coin100_100 = \<lparr>Label = ''coin'', Arity = 1, Guard = [gexp.Eq (V (I 1)) (L (Num 100))], Outputs = [L (Num 100)], Updates = []\<rparr>"
+
+definition selectPepsi :: transition where
+  "selectPepsi = \<lparr>Label = ''select'', Arity = 1, Guard = [gexp.Eq (V (I 1)) (L (Str ''pepsi''))], Outputs = [], Updates = []\<rparr>"
+
+definition vend_pepsi :: transition where
+  "vend_pepsi = \<lparr>Label = ''vend'', Arity = 0, Guard = [], Outputs = [L (Str ''pepsi'')], Updates = []\<rparr>"
+
+lemmas transitions = selectCoke_def coin50_50_def coin50_100_def vend_coke_def selectPepsi_def coin100_100_def vend_pepsi_def
+
+definition pta :: iEFSM where
+  "pta = {|(0, (0, 1), selectCoke),  (2, (1, 2), coin50_50), (4, (2, 3), coin50_100),  (5, (3, 4), vend_coke),
+                                                             (3, (1, 5), coin100_100), (6, (5, 6), vend_coke),
+           (1, (0, 7), selectPepsi), (7, (7, 8), coin50_50), (8, (8, 9), coin50_100),  (9, (9, 10), vend_pepsi)|}"
+
+lemma step_pta_selectPepsi: "step (tm pta) 0 Map.empty ''select'' [Str ''pepsi''] = Some (selectPepsi, 7, [], <>)"
+proof-
+  have possible_steps: "possible_steps (tm pta) 0 Map.empty ''select'' [Str ''pepsi''] = {|(7, selectPepsi)|}"
+    apply (simp add: possible_steps_def ffilter_def fimage_def fset_both_sides Abs_fset_inverse)
+    apply (simp add: tm_def pta_def Set.filter_def)
+    apply safe
+                      apply (simp_all add: transitions)
+    by force
+  show ?thesis
+    apply (simp add: step_def possible_steps)
+    by (simp add: selectPepsi_def)
+qed
+
+definition traces :: log where
+  "traces = [[(''select'', [Str ''coke''], []), (''coin'', [Num 50], [Num 50]), (''coin'', [Num 50], [Num 100]), (''vend'', [], [Str ''coke''])],
+             [(''select'', [Str ''coke''], []), (''coin'', [Num 100], [Num 100]), (''vend'', [], [Str ''coke''])],
+             [(''select'', [Str ''pepsi''], []), (''coin'', [Num 50], [Num 50]), (''coin'', [Num 50], [Num 100]), (''vend'', [], [Str ''pepsi''])]]"
+
+
+lemma build_pta: "toiEFSM (make_pta traces {||}) = pta"
+proof-
+ have step_coin50: "step {|((0, 1), \<lparr>Label = ''select'', Arity = Suc 0, Guard = [gexp.Eq (V (I 1)) (L (Str ''coke''))], Outputs = [], Updates = []\<rparr>)|} 1 Map.empty
+           ''coin'' [Num 50] = None"
+    proof-
+      have set_filter: "(Set.filter
+         (\<lambda>((origin, dest), t).
+             origin = 1 \<and>
+             Label t = ''coin'' \<and>
+             Suc 0 = Arity t \<and> apply_guards (Guard t) (case_vname (\<lambda>n. if n = 1 then Some (Num 50) else input2state [] (1 + 1) (I n)) Map.empty))
+         {((0, 1), \<lparr>Label = ''select'', Arity = Suc 0, Guard = [gexp.Eq (V (I 1)) (L (Str ''coke''))], Outputs = [], Updates = []\<rparr>)}) = {}"
+        by (simp add: Set.filter_def)
+      show ?thesis
+        by (simp add: step_def possible_steps_def ffilter_def set_filter)
+    qed
+    have step_coin50_2: "step
+           {|((1, 2), \<lparr>Label = ''coin'', Arity = Suc 0, Guard = [gexp.Eq (V (I 1)) (L (Num 50))], Outputs = [L (Num 50)], Updates = []\<rparr>),
+             ((0, 1), \<lparr>Label = ''select'', Arity = Suc 0, Guard = [gexp.Eq (V (I 1)) (L (Str ''coke''))], Outputs = [], Updates = []\<rparr>)|}
+           2 Map.empty ''coin'' [Num 50] = None"
+    proof-
+      have set_filter: "Set.filter
+         (\<lambda>((origin, dest), t).
+             origin = (2::nat) \<and>
+             Label t = ''coin'' \<and>
+             Suc 0 = Arity t \<and> apply_guards (Guard t) (case_vname (\<lambda>n. if n = 1 then Some (Num 50) else input2state [] (1 + 1) (I n)) Map.empty))
+         {((1, 2), \<lparr>Label = ''coin'', Arity = Suc 0, Guard = [gexp.Eq (V (I 1)) (L (Num 50))], Outputs = [L (Num 50)], Updates = []\<rparr>),
+          ((0, 1), \<lparr>Label = ''select'', Arity = Suc 0, Guard = [gexp.Eq (V (I 1)) (L (Str ''coke''))], Outputs = [], Updates = []\<rparr>)} = {}"
+        by (simp add: Set.filter_def)
+      show ?thesis
+        by (simp add: step_def possible_steps_def ffilter_def set_filter)
+    qed
+    have step_vend_coke: "step
+           {|((2, 3), \<lparr>Label = ''coin'', Arity = Suc 0, Guard = [gexp.Eq (V (I 1)) (L (Num 50))], Outputs = [L (Num 100)], Updates = []\<rparr>),
+             ((1, 2), \<lparr>Label = ''coin'', Arity = Suc 0, Guard = [gexp.Eq (V (I 1)) (L (Num 50))], Outputs = [L (Num 50)], Updates = []\<rparr>),
+             ((0, 1), \<lparr>Label = ''select'', Arity = Suc 0, Guard = [gexp.Eq (V (I 1)) (L (Str ''coke''))], Outputs = [], Updates = []\<rparr>)|}
+           3 Map.empty ''vend'' [] = None"
+    proof-
+      have set_filter: "Set.filter (\<lambda>((origin, dest), t). origin = (3::nat) \<and> Label t = ''vend'' \<and> Arity t = 0 \<and> apply_guards (Guard t) (case_vname Map.empty Map.empty))
+         {((2, 3), \<lparr>Label = ''coin'', Arity = Suc 0, Guard = [gexp.Eq (V (I 1)) (L (Num 50))], Outputs = [L (Num 100)], Updates = []\<rparr>),
+          ((1, 2), \<lparr>Label = ''coin'', Arity = Suc 0, Guard = [gexp.Eq (V (I 1)) (L (Num 50))], Outputs = [L (Num 50)], Updates = []\<rparr>),
+          ((0, 1), \<lparr>Label = ''select'', Arity = Suc 0, Guard = [gexp.Eq (V (I 1)) (L (Str ''coke''))], Outputs = [], Updates = []\<rparr>)} = {}"
+        by (simp add: Set.filter_def)
+      show ?thesis
+        by (simp add: step_def possible_steps_def ffilter_def set_filter)
+    qed
+    have step_selectCoke_2: "step
+                  {|((3, 4), \<lparr>Label = ''vend'', Arity = 0, Guard = [], Outputs = [L (Str ''coke'')], Updates = []\<rparr>),
+                    ((2, 3), \<lparr>Label = ''coin'', Arity = Suc 0, Guard = [gexp.Eq (V (I 1)) (L (Num 50))], Outputs = [L (Num 100)], Updates = []\<rparr>),
+                    ((1, 2), \<lparr>Label = ''coin'', Arity = Suc 0, Guard = [gexp.Eq (V (I 1)) (L (Num 50))], Outputs = [L (Num 50)], Updates = []\<rparr>),
+                    ((0, 1), \<lparr>Label = ''select'', Arity = Suc 0, Guard = [gexp.Eq (V (I 1)) (L (Str ''coke''))], Outputs = [], Updates = []\<rparr>)|}
+                  0 Map.empty ''select'' [Str ''coke''] = Some (selectCoke, 1, [], <>)"
+    proof-
+      have set_filter: "Set.filter
+          (\<lambda>((origin, dest), t).
+              origin = 0 \<and>
+              Label t = ''select'' \<and>
+              Suc 0 = Arity t \<and> apply_guards (Guard t) (case_vname (\<lambda>n. if n = 1 then Some (Str ''coke'') else input2state [] (1 + 1) (I n)) Map.empty))
+          {((3, 4), \<lparr>Label = ''vend'', Arity = 0, Guard = [], Outputs = [L (Str ''coke'')], Updates = []\<rparr>),
+           ((2, 3), \<lparr>Label = ''coin'', Arity = Suc 0, Guard = [gexp.Eq (V (I 1)) (L (Num 50))], Outputs = [L (Num 100)], Updates = []\<rparr>),
+           ((1, 2), \<lparr>Label = ''coin'', Arity = Suc 0, Guard = [gexp.Eq (V (I 1)) (L (Num 50))], Outputs = [L (Num 50)], Updates = []\<rparr>),
+           ((0, 1), \<lparr>Label = ''select'', Arity = Suc 0, Guard = [gexp.Eq (V (I 1)) (L (Str ''coke''))], Outputs = [], Updates = []\<rparr>)} = {((0, 1), selectCoke)}"
+        apply (simp add: Set.filter_def)
+        apply safe
+        by (simp_all add: selectCoke_def)
+      show ?thesis
+        apply (simp add: step_def possible_steps_def ffilter_def set_filter)
+        by (simp add: set_filter selectCoke_def)
+    qed
+    have step_coin100: "step
+                  {|((3, 4), \<lparr>Label = ''vend'', Arity = 0, Guard = [], Outputs = [L (Str ''coke'')], Updates = []\<rparr>),
+                    ((2, 3), \<lparr>Label = ''coin'', Arity = Suc 0, Guard = [gexp.Eq (V (I 1)) (L (Num 50))], Outputs = [L (Num 100)], Updates = []\<rparr>),
+                    ((1, 2), \<lparr>Label = ''coin'', Arity = Suc 0, Guard = [gexp.Eq (V (I 1)) (L (Num 50))], Outputs = [L (Num 50)], Updates = []\<rparr>),
+                    ((0, 1), \<lparr>Label = ''select'', Arity = Suc 0, Guard = [gexp.Eq (V (I 1)) (L (Str ''coke''))], Outputs = [], Updates = []\<rparr>)|}
+                  1 Map.empty ''coin'' [Num 100] = None"
+    proof-
+      have applyGuards: "\<not> apply_guards [gexp.Eq (V (I 1)) (L (Num 50))] (case_vname (\<lambda>n. if n = 1 then Some (Num 100) else input2state [] (1 + 1) (I n)) Map.empty)"
+        by simp
+      have set_filter: "Set.filter
+         (\<lambda>((origin::nat, dest), t).
+             origin = 1 \<and>
+             Label t = ''coin'' \<and>
+             Suc 0 = Arity t \<and> apply_guards (Guard t) (case_vname (\<lambda>n. if n = 1 then Some (Num 100) else input2state [] (1 + 1) (I n)) Map.empty))
+         {((3, 4), \<lparr>Label = ''vend'', Arity = 0, Guard = [], Outputs = [L (Str ''coke'')], Updates = []\<rparr>),
+          ((2, 3), \<lparr>Label = ''coin'', Arity = Suc 0, Guard = [gexp.Eq (V (I 1)) (L (Num 50))], Outputs = [L (Num 100)], Updates = []\<rparr>),
+          ((1, 2), \<lparr>Label = ''coin'', Arity = Suc 0, Guard = [gexp.Eq (V (I 1)) (L (Num 50))], Outputs = [L (Num 50)], Updates = []\<rparr>),
+          ((0, 1), \<lparr>Label = ''select'', Arity = Suc 0, Guard = [gexp.Eq (V (I 1)) (L (Str ''coke''))], Outputs = [], Updates = []\<rparr>)} = {}"
+        apply (simp add: Set.filter_def)
+        apply clarify
+        using applyGuards
+        by (metis (no_types, lifting) select_convs(3))
+      show ?thesis
+        by (simp add: step_def possible_steps_def ffilter_def set_filter)
+    qed
+    have step_vend_coke_2: "step
+                  {|((1, 5), \<lparr>Label = ''coin'', Arity = Suc 0, Guard = [gexp.Eq (V (I 1)) (L (Num 100))], Outputs = [L (Num 100)], Updates = []\<rparr>),
+                    ((3, 4), \<lparr>Label = ''vend'', Arity = 0, Guard = [], Outputs = [L (Str ''coke'')], Updates = []\<rparr>),
+                    ((2, 3), \<lparr>Label = ''coin'', Arity = Suc 0, Guard = [gexp.Eq (V (I 1)) (L (Num 50))], Outputs = [L (Num 100)], Updates = []\<rparr>),
+                    ((1, 2), \<lparr>Label = ''coin'', Arity = Suc 0, Guard = [gexp.Eq (V (I 1)) (L (Num 50))], Outputs = [L (Num 50)], Updates = []\<rparr>),
+                    ((0, 1), \<lparr>Label = ''select'', Arity = Suc 0, Guard = [gexp.Eq (V (I 1)) (L (Str ''coke''))], Outputs = [], Updates = []\<rparr>)|}
+                  5 Map.empty ''vend'' [] = None"
+    proof-
+      have set_filter: "Set.filter (\<lambda>((origin::nat, dest), t). origin = 5 \<and> Label t = ''vend'' \<and> Arity t = 0 \<and> apply_guards (Guard t) (case_vname Map.empty Map.empty))
+         {((1, 5), \<lparr>Label = ''coin'', Arity = Suc 0, Guard = [gexp.Eq (V (I 1)) (L (Num 100))], Outputs = [L (Num 100)], Updates = []\<rparr>),
+          ((3, 4), \<lparr>Label = ''vend'', Arity = 0, Guard = [], Outputs = [L (Str ''coke'')], Updates = []\<rparr>),
+          ((2, 3), \<lparr>Label = ''coin'', Arity = Suc 0, Guard = [gexp.Eq (V (I 1)) (L (Num 50))], Outputs = [L (Num 100)], Updates = []\<rparr>),
+          ((1, 2), \<lparr>Label = ''coin'', Arity = Suc 0, Guard = [gexp.Eq (V (I 1)) (L (Num 50))], Outputs = [L (Num 50)], Updates = []\<rparr>),
+          ((0, 1), \<lparr>Label = ''select'', Arity = Suc 0, Guard = [gexp.Eq (V (I 1)) (L (Str ''coke''))], Outputs = [], Updates = []\<rparr>)} = {}"
+        by (simp add: Set.filter_def)
+      show ?thesis
+        by (simp add: step_def possible_steps_def ffilter_def set_filter)
+    qed
+    have step_select_pepsi: "step
+           {|((5, 6), \<lparr>Label = ''vend'', Arity = 0, Guard = [], Outputs = [L (Str ''coke'')], Updates = []\<rparr>),
+             ((1, 5), \<lparr>Label = ''coin'', Arity = Suc 0, Guard = [gexp.Eq (V (I 1)) (L (Num 100))], Outputs = [L (Num 100)], Updates = []\<rparr>),
+             ((3, 4), \<lparr>Label = ''vend'', Arity = 0, Guard = [], Outputs = [L (Str ''coke'')], Updates = []\<rparr>),
+             ((2, 3), \<lparr>Label = ''coin'', Arity = Suc 0, Guard = [gexp.Eq (V (I 1)) (L (Num 50))], Outputs = [L (Num 100)], Updates = []\<rparr>),
+             ((1, 2), \<lparr>Label = ''coin'', Arity = Suc 0, Guard = [gexp.Eq (V (I 1)) (L (Num 50))], Outputs = [L (Num 50)], Updates = []\<rparr>),
+             ((0, 1), \<lparr>Label = ''select'', Arity = Suc 0, Guard = [gexp.Eq (V (I 1)) (L (Str ''coke''))], Outputs = [], Updates = []\<rparr>)|}
+           0 Map.empty ''select'' [Str ''pepsi''] = None"
+    proof-
+      have applyGuards: "\<not>apply_guards [gexp.Eq (V (I 1)) (L (Str ''coke''))] (case_vname (\<lambda>n. if n = 1 then Some (Str ''pepsi'') else input2state [] (1 + 1) (I n)) Map.empty)"
+        by simp
+      have set_filter: "Set.filter
+         (\<lambda>((origin::nat, dest::nat), t).
+             origin = 0 \<and>
+             Label t = ''select'' \<and>
+             Suc 0 = Arity t \<and> apply_guards (Guard t) (case_vname (\<lambda>n. if n = 1 then Some (Str ''pepsi'') else input2state [] (1 + 1) (I n)) Map.empty))
+         {((5, 6), \<lparr>Label = ''vend'', Arity = 0, Guard = [], Outputs = [L (Str ''coke'')], Updates = []\<rparr>),
+          ((1, 5), \<lparr>Label = ''coin'', Arity = Suc 0, Guard = [gexp.Eq (V (I 1)) (L (Num 100))], Outputs = [L (Num 100)], Updates = []\<rparr>),
+          ((3, 4), \<lparr>Label = ''vend'', Arity = 0, Guard = [], Outputs = [L (Str ''coke'')], Updates = []\<rparr>),
+          ((2, 3), \<lparr>Label = ''coin'', Arity = Suc 0, Guard = [gexp.Eq (V (I 1)) (L (Num 50))], Outputs = [L (Num 100)], Updates = []\<rparr>),
+          ((1, 2), \<lparr>Label = ''coin'', Arity = Suc 0, Guard = [gexp.Eq (V (I 1)) (L (Num 50))], Outputs = [L (Num 50)], Updates = []\<rparr>),
+          ((0, 1), \<lparr>Label = ''select'', Arity = Suc 0, Guard = [gexp.Eq (V (I 1)) (L (Str ''coke''))], Outputs = [], Updates = []\<rparr>)} = {}"
+        apply (simp add: Set.filter_def)
+        apply clarify
+        apply simp
+        by (metis (no_types, lifting) applyGuards select_convs(3))
+      show ?thesis
+        by (simp add: step_def possible_steps_def ffilter_def set_filter)
+    qed
+    have step_coin50_3:  "step
+           {|((0, 7), \<lparr>Label = ''select'', Arity = Suc 0, Guard = [gexp.Eq (V (I 1)) (L (Str ''pepsi''))], Outputs = [], Updates = []\<rparr>),
+             ((5, 6), \<lparr>Label = ''vend'', Arity = 0, Guard = [], Outputs = [L (Str ''coke'')], Updates = []\<rparr>),
+             ((1, 5), \<lparr>Label = ''coin'', Arity = Suc 0, Guard = [gexp.Eq (V (I 1)) (L (Num 100))], Outputs = [L (Num 100)], Updates = []\<rparr>),
+             ((3, 4), \<lparr>Label = ''vend'', Arity = 0, Guard = [], Outputs = [L (Str ''coke'')], Updates = []\<rparr>),
+             ((2, 3), \<lparr>Label = ''coin'', Arity = Suc 0, Guard = [gexp.Eq (V (I 1)) (L (Num 50))], Outputs = [L (Num 100)], Updates = []\<rparr>),
+             ((1, 2), \<lparr>Label = ''coin'', Arity = Suc 0, Guard = [gexp.Eq (V (I 1)) (L (Num 50))], Outputs = [L (Num 50)], Updates = []\<rparr>),
+             ((0, 1), \<lparr>Label = ''select'', Arity = Suc 0, Guard = [gexp.Eq (V (I 1)) (L (Str ''coke''))], Outputs = [], Updates = []\<rparr>)|}
+           7 Map.empty ''coin'' [Num 50] = None"
+    proof-
+      have set_filter: "Set.filter
+         (\<lambda>((origin::nat, dest::nat), t).
+             origin = 7 \<and>
+             Label t = ''coin'' \<and>
+             Suc 0 = Arity t \<and> apply_guards (Guard t) (case_vname (\<lambda>n. if n = 1 then Some (Num 50) else input2state [] (1 + 1) (I n)) Map.empty))
+         {((0, 7), \<lparr>Label = ''select'', Arity = Suc 0, Guard = [gexp.Eq (V (I 1)) (L (Str ''pepsi''))], Outputs = [], Updates = []\<rparr>),
+          ((5, 6), \<lparr>Label = ''vend'', Arity = 0, Guard = [], Outputs = [L (Str ''coke'')], Updates = []\<rparr>),
+          ((1, 5), \<lparr>Label = ''coin'', Arity = Suc 0, Guard = [gexp.Eq (V (I 1)) (L (Num 100))], Outputs = [L (Num 100)], Updates = []\<rparr>),
+          ((3, 4), \<lparr>Label = ''vend'', Arity = 0, Guard = [], Outputs = [L (Str ''coke'')], Updates = []\<rparr>),
+          ((2, 3), \<lparr>Label = ''coin'', Arity = Suc 0, Guard = [gexp.Eq (V (I 1)) (L (Num 50))], Outputs = [L (Num 100)], Updates = []\<rparr>),
+          ((1, 2), \<lparr>Label = ''coin'', Arity = Suc 0, Guard = [gexp.Eq (V (I 1)) (L (Num 50))], Outputs = [L (Num 50)], Updates = []\<rparr>),
+          ((0, 1), \<lparr>Label = ''select'', Arity = Suc 0, Guard = [gexp.Eq (V (I 1)) (L (Str ''coke''))], Outputs = [], Updates = []\<rparr>)} = {}"
+        by (simp add: Set.filter_def)
+    show ?thesis
+      by (simp add: step_def possible_steps_def ffilter_def set_filter)
+  qed
+  have step_coin50_4: "step
+           {|((7, 8), \<lparr>Label = ''coin'', Arity = Suc 0, Guard = [gexp.Eq (V (I 1)) (L (Num 50))], Outputs = [L (Num 50)], Updates = []\<rparr>),
+             ((0, 7), \<lparr>Label = ''select'', Arity = Suc 0, Guard = [gexp.Eq (V (I 1)) (L (Str ''pepsi''))], Outputs = [], Updates = []\<rparr>),
+             ((5, 6), \<lparr>Label = ''vend'', Arity = 0, Guard = [], Outputs = [L (Str ''coke'')], Updates = []\<rparr>),
+             ((1, 5), \<lparr>Label = ''coin'', Arity = Suc 0, Guard = [gexp.Eq (V (I 1)) (L (Num 100))], Outputs = [L (Num 100)], Updates = []\<rparr>),
+             ((3, 4), \<lparr>Label = ''vend'', Arity = 0, Guard = [], Outputs = [L (Str ''coke'')], Updates = []\<rparr>),
+             ((2, 3), \<lparr>Label = ''coin'', Arity = Suc 0, Guard = [gexp.Eq (V (I 1)) (L (Num 50))], Outputs = [L (Num 100)], Updates = []\<rparr>),
+             ((1, 2), \<lparr>Label = ''coin'', Arity = Suc 0, Guard = [gexp.Eq (V (I 1)) (L (Num 50))], Outputs = [L (Num 50)], Updates = []\<rparr>),
+             ((0, 1), \<lparr>Label = ''select'', Arity = Suc 0, Guard = [gexp.Eq (V (I 1)) (L (Str ''coke''))], Outputs = [], Updates = []\<rparr>)|}
+           8 Map.empty ''coin'' [Num 50] = None"
+  proof-
+    have set_filter: "Set.filter
+         (\<lambda>((origin::nat, dest::nat), t).
+             origin = 8 \<and>
+             Label t = ''coin'' \<and>
+             Suc 0 = Arity t \<and> apply_guards (Guard t) (case_vname (\<lambda>n. if n = 1 then Some (Num 50) else input2state [] (1 + 1) (I n)) Map.empty))
+         {((7, 8), \<lparr>Label = ''coin'', Arity = Suc 0, Guard = [gexp.Eq (V (I 1)) (L (Num 50))], Outputs = [L (Num 50)], Updates = []\<rparr>),
+          ((0, 7), \<lparr>Label = ''select'', Arity = Suc 0, Guard = [gexp.Eq (V (I 1)) (L (Str ''pepsi''))], Outputs = [], Updates = []\<rparr>),
+          ((5, 6), \<lparr>Label = ''vend'', Arity = 0, Guard = [], Outputs = [L (Str ''coke'')], Updates = []\<rparr>),
+          ((1, 5), \<lparr>Label = ''coin'', Arity = Suc 0, Guard = [gexp.Eq (V (I 1)) (L (Num 100))], Outputs = [L (Num 100)], Updates = []\<rparr>),
+          ((3, 4), \<lparr>Label = ''vend'', Arity = 0, Guard = [], Outputs = [L (Str ''coke'')], Updates = []\<rparr>),
+          ((2, 3), \<lparr>Label = ''coin'', Arity = Suc 0, Guard = [gexp.Eq (V (I 1)) (L (Num 50))], Outputs = [L (Num 100)], Updates = []\<rparr>),
+          ((1, 2), \<lparr>Label = ''coin'', Arity = Suc 0, Guard = [gexp.Eq (V (I 1)) (L (Num 50))], Outputs = [L (Num 50)], Updates = []\<rparr>),
+          ((0, 1), \<lparr>Label = ''select'', Arity = Suc 0, Guard = [gexp.Eq (V (I 1)) (L (Str ''coke''))], Outputs = [], Updates = []\<rparr>)} = {}"
+      by (simp add: Set.filter_def)
+    show ?thesis
+      by (simp add: step_def possible_steps_def ffilter_def set_filter)
+  qed
+  have step_vend_pepsi: "step
+           {|((8, 9), \<lparr>Label = ''coin'', Arity = Suc 0, Guard = [gexp.Eq (V (I 1)) (L (Num 50))], Outputs = [L (Num 100)], Updates = []\<rparr>),
+             ((7, 8), \<lparr>Label = ''coin'', Arity = Suc 0, Guard = [gexp.Eq (V (I 1)) (L (Num 50))], Outputs = [L (Num 50)], Updates = []\<rparr>),
+             ((0, 7), \<lparr>Label = ''select'', Arity = Suc 0, Guard = [gexp.Eq (V (I 1)) (L (Str ''pepsi''))], Outputs = [], Updates = []\<rparr>),
+             ((5, 6), \<lparr>Label = ''vend'', Arity = 0, Guard = [], Outputs = [L (Str ''coke'')], Updates = []\<rparr>),
+             ((1, 5), \<lparr>Label = ''coin'', Arity = Suc 0, Guard = [gexp.Eq (V (I 1)) (L (Num 100))], Outputs = [L (Num 100)], Updates = []\<rparr>),
+             ((3, 4), \<lparr>Label = ''vend'', Arity = 0, Guard = [], Outputs = [L (Str ''coke'')], Updates = []\<rparr>),
+             ((2, 3), \<lparr>Label = ''coin'', Arity = Suc 0, Guard = [gexp.Eq (V (I 1)) (L (Num 50))], Outputs = [L (Num 100)], Updates = []\<rparr>),
+             ((1, 2), \<lparr>Label = ''coin'', Arity = Suc 0, Guard = [gexp.Eq (V (I 1)) (L (Num 50))], Outputs = [L (Num 50)], Updates = []\<rparr>),
+             ((0, 1), \<lparr>Label = ''select'', Arity = Suc 0, Guard = [gexp.Eq (V (I 1)) (L (Str ''coke''))], Outputs = [], Updates = []\<rparr>)|}
+           9 Map.empty ''vend'' [] = None"
+  proof-
+    have set_filter: "Set.filter (\<lambda>((origin::nat, dest::nat), t). origin = 9 \<and> Label t = ''vend'' \<and> Arity t = 0 \<and> apply_guards (Guard t) (case_vname Map.empty Map.empty))
+         {((8, 9), \<lparr>Label = ''coin'', Arity = Suc 0, Guard = [gexp.Eq (V (I 1)) (L (Num 50))], Outputs = [L (Num 100)], Updates = []\<rparr>),
+         ((7, 8), \<lparr>Label = ''coin'', Arity = Suc 0, Guard = [gexp.Eq (V (I 1)) (L (Num 50))], Outputs = [L (Num 50)], Updates = []\<rparr>),
+         ((0, 7), \<lparr>Label = ''select'', Arity = Suc 0, Guard = [gexp.Eq (V (I 1)) (L (Str ''pepsi''))], Outputs = [], Updates = []\<rparr>),
+         ((5, 6), \<lparr>Label = ''vend'', Arity = 0, Guard = [], Outputs = [L (Str ''coke'')], Updates = []\<rparr>),
+         ((1, 5), \<lparr>Label = ''coin'', Arity = Suc 0, Guard = [gexp.Eq (V (I 1)) (L (Num 100))], Outputs = [L (Num 100)], Updates = []\<rparr>),
+         ((3, 4), \<lparr>Label = ''vend'', Arity = 0, Guard = [], Outputs = [L (Str ''coke'')], Updates = []\<rparr>),
+         ((2, 3), \<lparr>Label = ''coin'', Arity = Suc 0, Guard = [gexp.Eq (V (I 1)) (L (Num 50))], Outputs = [L (Num 100)], Updates = []\<rparr>),
+         ((1, 2), \<lparr>Label = ''coin'', Arity = Suc 0, Guard = [gexp.Eq (V (I 1)) (L (Num 50))], Outputs = [L (Num 50)], Updates = []\<rparr>),
+         ((0, 1), \<lparr>Label = ''select'', Arity = Suc 0, Guard = [gexp.Eq (V (I 1)) (L (Str ''coke''))], Outputs = [], Updates = []\<rparr>)} = {}"
+      by (simp add: Set.filter_def)
+    show ?thesis
+      by (simp add: step_def possible_steps_def ffilter_def set_filter)
+  qed
+  have select_coke: " \<lparr>Label = ''select'', Arity = Suc 0, Guard = [gexp.Eq (V (I 1)) (L (Str ''coke''))], Outputs = [], Updates = []\<rparr> = selectCoke"
+    by (simp add: selectCoke_def)
+  have coin50_50: "\<lparr>Label = ''coin'', Arity = Suc 0, Guard = [gexp.Eq (V (I 1)) (L (Num 50))], Outputs = [L (Num 50)], Updates = []\<rparr> = coin50_50"
+    by (simp add: coin50_50_def)
+  have coin100_100: " \<lparr>Label = ''coin'', Arity = Suc 0, Guard = [gexp.Eq (V (I 1)) (L (Num 100))], Outputs = [L (Num 100)], Updates = []\<rparr> = coin100_100"
+    by (simp add: coin100_100_def)
+  have coin50_100: "\<lparr>Label = ''coin'', Arity = Suc 0, Guard = [gexp.Eq (V (I 1)) (L (Num 50))], Outputs = [L (Num 100)], Updates = []\<rparr> = coin50_100"
+    by (simp add: coin50_100_def)
+  have selectPepsi: "\<lparr>Label = ''select'', Arity = Suc 0, Guard = [gexp.Eq (V (I 1)) (L (Str ''pepsi''))], Outputs = [], Updates = []\<rparr> = selectPepsi"
+    by (simp add: selectPepsi_def)
+  have vendCoke: "\<lparr>Label = ''vend'', Arity = 0, Guard = [], Outputs = [L (Str ''coke'')], Updates = []\<rparr> = vend_coke"
+    by (simp add: vend_coke_def)
+  have vendPepsi: "\<lparr>Label = ''vend'', Arity = 0, Guard = [], Outputs = [L (Str ''pepsi'')], Updates = []\<rparr> = vend_pepsi"
+    by (simp add: vend_pepsi_def)
+  have sorted_list_of_fset: "sorted_list_of_fset
+         {|((9::nat, 10::nat), vend_pepsi), ((8, 9), coin50_100), ((7, 8), coin50_50), ((0, 7), selectPepsi), ((5, 6), vend_coke),
+           ((1, 5), coin100_100), ((3, 4), vend_coke), ((2, 3), coin50_100), ((1, 2), coin50_50), ((0, 1), selectCoke)|} = [((0, 1), selectCoke), ((0, 7), selectPepsi), ((1, 2), coin50_50), ((1, 5), coin100_100), ((2, 3), coin50_100), ((3, 4), vend_coke),
+     ((5, 6), vend_coke), ((7, 8), coin50_50), ((8, 9), coin50_100), ((9, 10), vend_pepsi)]"
+    by (simp add: sorted_list_of_fset_def )
+  show ?thesis
+    apply (simp add: make_pta_def traces_def)
+    apply (simp add: step_coin50 step_coin50_2 step_vend_coke
+                      step_selectCoke_2 step_coin100 step_vend_coke_2
+                      step_select_pepsi step_coin50_3 step_coin50_4 step_vend_pepsi)
+    apply (simp add: select_coke coin50_50 coin100_100 coin50_100 selectPepsi vendCoke vendPepsi)
+    apply (simp add: toiEFSM_def toiEFSM_aux_def)
+    apply (simp add: sorted_list_of_fset pta_def)
+    by auto
+qed
+
+definition filtered_pairs :: "(nat \<times> nat) set" where
+  "filtered_pairs = {(9, 10), (8, 10), (8, 9), (7, 10), (7, 9), (7, 8), (6, 10), (6, 9), (6, 8), (6, 7), (5, 10), (5, 9), (5, 8), (5, 7), (5, 6), (4, 10),
+  (4, 9), (4, 8), (4, 7), (4, 6), (4, 5), (3, 10), (3, 9), (3, 8), (3, 7), (3, 6), (3, 5), (3, 4), (2, 10), (2, 9), (2, 8), (2, 7), (2, 6),
+  (2, 5), (2, 4), (2, 3), (1, 10), (1, 9), (1, 8), (1, 7), (1, 6), (1, 5), (1, 4), (1, 3), (1, 2), (0, 10), (0, 9), (0, 8), (0, 7), (0, 6),
+  (0, 5), (0, 4), (0, 3), (0, 2), (0, 1)}"
+
+lemma scoring_1: "sorted_list_of_fset (score pta naive_score) = [(0, 0, 1), (0, 0, 2), (0, 0, 3), (0, 0, 4), (0, 0, 5), (0, 0, 6), (0, 0, 7), (0, 0, 8), (0, 0, 9), (0, 0, 10), (0, 1, 3), (0, 1, 4),
+     (0, 1, 5), (0, 1, 6), (0, 1, 9), (0, 1, 10), (0, 2, 3), (0, 2, 4), (0, 2, 5), (0, 2, 6), (0, 2, 9), (0, 2, 10), (0, 3, 4), (0, 3, 6),
+     (0, 3, 7), (0, 3, 8), (0, 3, 10), (0, 4, 5), (0, 4, 6), (0, 4, 7), (0, 4, 8), (0, 4, 9), (0, 4, 10), (0, 5, 6), (0, 5, 7), (0, 5, 8),
+     (0, 5, 10), (0, 6, 7), (0, 6, 8), (0, 6, 9), (0, 6, 10), (0, 7, 9), (0, 7, 10), (0, 8, 9), (0, 8, 10), (0, 9, 10), (1, 2, 7), (1, 2, 8),
+     (1, 3, 5), (1, 3, 9), (1, 5, 9), (1, 7, 8), (2, 1, 2), (2, 1, 7), (2, 1, 8)]"
+proof-
+  have S_pta: "S pta = {|0, 1, 2, 3, 4, 5, 6, 7, 8, 9, 10|}"
+    apply (simp add: S_def pta_def)
+    by auto
+  have fset_S: "fset {|0, 1, 2, 3, 4, 5, 6, 7, 8, 9, 10|} = {0, 1, 2, 3, 4, 5, 6, 7, 8, 9, 10}"
+    by (metis bot_fset.rep_eq finsert.rep_eq)
+  have ffilter: "ffilter (\<lambda>(x, y). x < y) (Inference.S pta |\<times>| Inference.S pta) = Abs_fset filtered_pairs"
+    apply (simp add: filtered_pairs_def ffilter_def fset_both_sides Abs_fset_inverse fprod_def)
+    apply (simp only: S_pta fprod_equiv fset_S Set.filter_def)
+    apply standard
+     apply clarify
+     apply (case_tac "a=10")
+      apply auto[1]
+      apply simp
+      apply (case_tac "a=9")
+       apply auto[1]
+      apply simp
+      apply (case_tac "a=8")
+       apply auto[1]
+      apply simp
+      apply (case_tac "a=7")
+       apply auto[1]
+      apply simp
+      apply (case_tac "a=6")
+       apply auto[1]
+      apply simp
+      apply (case_tac "a=5")
+       apply auto[1]
+      apply simp
+      apply (case_tac "a=4")
+       apply auto[1]
+      apply simp
+      apply (case_tac "a=3")
+       apply auto[1]
+      apply simp
+      apply (case_tac "a=2")
+        apply auto[1]
+      apply simp
+      apply (case_tac "a=1")
+      apply auto[1]
+     apply simp
+    apply clarify
+    apply safe
+    by auto
+  have Two_nat_def: "2 = Suc (Suc 0)"
+    by simp
+  have scores: "score pta naive_score = {|(0, 9, 10), (0, 8, 10), (0, 8, 9), (0, 7, 10), (0, 7, 9), (1, 7, 8), (0, 6, 10), (0, 6, 9), (0, 6, 8), (0, 6, 7), (0, 5, 10),
+     (1, 5, 9), (0, 5, 8), (0, 5, 7), (0, 5, 6), (0, 4, 10), (0, 4, 9), (0, 4, 8), (0, 4, 7), (0, 4, 6), (0, 4, 5), (0, 3, 10),
+     (1, 3, 9), (0, 3, 8), (0, 3, 7), (0, 3, 6), (1, 3, 5), (0, 3, 4), (0, 2, 10), (0, 2, 9), (1, 2, 8), (1, 2, 7),
+     (0, 2, 6), (0, 2, 5), (0, 2, 4), (0, 2, 3), (0, 1, 10), (0, 1, 9), (2, 1, 8), (2, 1, 7), (0, 1, 6), (0, 1, 5),
+     (0, 1, 4), (0, 1, 3), (2, 1, 2), (0, 0, 10), (0, 0, 9), (0, 0, 8), (0, 0, 7), (0, 0, 6), (0, 0, 5), (0, 0, 4), (0, 0, 3),
+     (0, 0, 2), (0, 0, 1)|}"
+    apply (simp add: score_def ffilter filtered_pairs_def)
+    apply (simp add: outgoing_transitions_def pta_def fimage_def)
+    apply (simp add: naive_score_empty set_equiv)
+    apply (simp add: naive_score_def fprod_def)
+    apply (simp add: transitions Abs_fset_inverse)
+    by (simp add: One_nat_def Two_nat_def)
+  show ?thesis
+    by (simp add: scores sorted_list_of_fset_def)
+qed
+
+lemmas possible_steps_fst = possible_steps_def ffilter_def fimage_def fset_both_sides Abs_fset_inverse
+
+lemma step_pta_coin50_7: "step (tm pta) 7 r ''coin'' [Num 50] = Some (coin50_50, 8, [Some (Num 50)], r)"
+proof-
+  have possible_steps: "possible_steps (tm pta) 7 r ''coin'' [Num 50] = {|(8, coin50_50)|}"
+    apply (simp add: possible_steps_fst)
+    apply (simp add: Set.filter_def tm_def pta_def)
+    apply safe
+                     apply (simp_all add: transitions)
+    by force
+  show ?thesis
+    apply (simp add: step_def possible_steps)
+    by (simp add: coin50_50_def)
+qed
+
+lemma step_pta_coin50_1: "step (tm pta) 1 r ''coin'' [Num 50] = Some (coin50_50, 2, [Some (Num 50)], r)"
+proof-
+  have possible_steps: "possible_steps (tm pta) 1 r ''coin'' [Num 50] = {|(2, coin50_50)|}"
+    apply (simp add: possible_steps_fst)
+    apply (simp add: Set.filter_def tm_def pta_def)
+    apply safe
+                     apply (simp_all add: transitions)
+    by force
+  show ?thesis
+    apply (simp add: step_def possible_steps)
+    by (simp add: coin50_50_def)
+qed
+
+lemma step_pta_vend_5: "step (tm pta) 5 r ''vend'' [] = Some (vend_coke, 6, [Some (Str ''coke'')], r)"
+proof-
+  have possible_steps: "possible_steps (tm pta) 5 r ''vend'' [] = {|(6, vend_coke)|}"
+    apply (simp add: possible_steps_fst)
+    apply (simp add: Set.filter_def tm_def pta_def)
+    apply safe
+                     apply (simp_all add: transitions)
+    by force
+  show ?thesis
+    apply (simp add: step_def possible_steps)
+    by (simp add: transitions)
+qed
+
+lemma step_pta_coin100_1: "step (tm pta) 1 r ''coin'' [Num 100] = Some (coin100_100, 5, [Some (Num 100)], r)"
+proof-
+  have possible_steps: "possible_steps (tm pta) 1 r ''coin'' [Num 100] = {|(5, coin100_100)|}"
+    apply (simp add: possible_steps_fst)
+    apply (simp add: Set.filter_def tm_def pta_def)
+    apply safe
+                     apply (simp_all add: transitions)
+    by force
+  show ?thesis
+    apply (simp add: step_def possible_steps)
+    by (simp add: coin100_100_def)
+qed
+
+lemma step_pta_coin50_2: "step (tm pta) 2 r ''coin'' [Num 50] = Some (coin50_100, 3, [Some (Num 100)], r)"
+proof-
+  have possible_steps: "possible_steps (tm pta) 2 r ''coin'' [Num 50] = {|(3, coin50_100)|}"
+    apply (simp add: possible_steps_fst)
+    apply (simp add: Set.filter_def tm_def pta_def)
+    apply safe
+                     apply (simp_all add: transitions)
+    by force
+  show ?thesis
+    apply (simp add: step_def possible_steps)
+    by (simp add: coin50_100_def)
+qed
+
+lemma step_pta_coin50_8: "step (tm pta) 8 r ''coin'' [Num 50] = Some (coin50_100, 9, [Some (Num 100)], r)"
+proof-
+  have possible_steps: "possible_steps (tm pta) 8 r ''coin'' [Num 50] = {|(9, coin50_100)|}"
+    apply (simp add: possible_steps_fst)
+    apply (simp add: Set.filter_def tm_def pta_def)
+    apply safe
+                     apply (simp_all add: transitions)
+    by force
+  show ?thesis
+    apply (simp add: step_def possible_steps)
+    by (simp add: coin50_100_def)
+qed
+
+lemma step_pta_vend_3: "step (tm pta) 3 r ''vend'' [] = Some (vend_coke, 4, [Some (Str ''coke'')], r)"
+proof-
+  have possible_steps: "possible_steps (tm pta) 3 r ''vend'' [] = {|(4, vend_coke)|}"
+    apply (simp add: possible_steps_fst)
+    apply (simp add: Set.filter_def tm_def pta_def)
+    apply safe
+                     apply (simp_all add: transitions)
+    by force
+  show ?thesis
+    apply (simp add: step_def possible_steps)
+    by (simp add: vend_coke_def)
+qed
+
+lemma step_pta_vend_9: "step (tm pta) 9 r ''vend'' [] = Some (vend_pepsi, 10, [Some (Str ''pepsi'')], r)"
+proof-
+  have possible_steps: "possible_steps (tm pta) 9 r ''vend'' [] = {|(10, vend_pepsi)|}"
+    apply (simp add: possible_steps_fst)
+    apply (simp add: Set.filter_def tm_def pta_def)
+    apply safe
+                     apply (simp_all add: transitions)
+    by force
+  show ?thesis
+    apply (simp add: step_def possible_steps)
+    by (simp add: vend_pepsi_def)
+qed
+
+definition merged_1_8 :: iEFSM where
+  "merged_1_8 = {|
+(0, (0, 1), selectCoke),
+(1, (0, 7), selectPepsi),
+(2, (1, 2), coin50_50),
+(3, (1, 5), coin100_100),
+(4, (2, 3), coin50_100),
+(5, (3, 4), vend_coke),
+(6, (5, 6), vend_coke),
+(7, (7, 1), coin50_50),
+(8, (1, 9), coin50_100),
+(9, (9, 10), vend_pepsi)
+|}"
+
+definition merged_2_9 :: iEFSM where
+  "merged_2_9 = {|(0, (0, 1), selectCoke), (1, (0, 7), selectPepsi), (2, (1, 2), coin50_50), (3, (1, 5), coin100_100), (4, (2, 3), coin50_100),
+      (5, (3, 4), vend_coke), (6, (5, 6), vend_coke), (7, (7, 1), coin50_50), (8, (1, 2), coin50_100), (9, (2, 10), vend_pepsi)|}"
+
+lemma merge_states_2_9: "merge_states 2 9 merged_1_8 = merged_2_9"
+  by (simp add: merge_states_def merge_states_aux_def merged_1_8_def merged_2_9_def)
+
+lemma step_merged_2_9_selectPepsi: "step (tm merged_2_9) 0 Map.empty ''select'' [Str ''pepsi''] = Some (selectPepsi, 7, [], <>)"
+proof-
+  have possible_steps: "possible_steps (tm merged_2_9) 0 Map.empty ''select'' [Str ''pepsi''] = {|(7, selectPepsi)|}"
+    apply (simp add: possible_steps_fst)
+    apply (simp add: tm_def merged_2_9_def Set.filter_def)
+    apply safe
+                      apply (simp_all add: transitions)
+    by force
+  show ?thesis
+    apply (simp add: step_def possible_steps)
+    by (simp add: selectPepsi_def)
+qed
+
+lemma step_merged_2_9_coin50_7: "step (tm merged_2_9) 7 r ''coin'' [Num 50] = Some (coin50_50, 1, [Some (Num 50)], r)"
+proof-
+  have possible_steps: "possible_steps (tm merged_2_9) 7 r ''coin'' [Num 50] = {|(1, coin50_50)|}"
+    apply (simp add: possible_steps_fst)
+    apply (simp add: tm_def merged_2_9_def Set.filter_def)
+    apply safe
+                      apply (simp_all add: transitions)
+    by force
+  show ?thesis
+    apply (simp add: step_def possible_steps)
+    by (simp add: coin50_50_def)
+qed
+
+lemma posterior_selectPepsi: "posterior \<lbrakk>\<rbrakk> selectPepsi = \<lbrakk>\<rbrakk>"
+proof-
+  have consistent_medial: "consistent (medial \<lbrakk>\<rbrakk> (Guard selectPepsi))"
+    apply (simp add: selectPepsi_def consistent_def)
+    apply (rule_tac x="<I 1 := Str ''pepsi''>" in exI)
+    by (simp add: consistent_empty_4)
+  show ?thesis
+    apply (simp add: posterior_def Let_def consistent_medial)
+    by (simp add: selectPepsi_def)
+qed
+
+lemma posterior_selectCoke: "posterior \<lbrakk>\<rbrakk> selectCoke = \<lbrakk>\<rbrakk>"
+proof-
+  have consistent_medial: "consistent (medial \<lbrakk>\<rbrakk> (Guard selectCoke))"
+    apply (simp add: selectCoke_def consistent_def)
+    apply (rule_tac x="<I 1 := Str ''coke''>" in exI)
+    by (simp add: consistent_empty_4)
+  show ?thesis
+    apply (simp add: posterior_def Let_def consistent_medial)
+    by (simp add: selectCoke_def)
+qed
+
+lemma posterior_coin50_50: "posterior \<lbrakk>\<rbrakk> coin50_50 = \<lbrakk>\<rbrakk>"
+proof-
+  have consistent_medial: "consistent (medial \<lbrakk>\<rbrakk> (Guard coin50_50))"
+    apply (simp add: coin50_50_def consistent_def)
+    apply (rule_tac x="<I 1 := Num 50>" in exI)
+    by (simp add: consistent_empty_4)
+  show ?thesis
+    apply (simp add: posterior_def Let_def consistent_medial)
+    by (simp add: coin50_50_def)
+qed
+
+lemma posterior_coin50_100: "posterior \<lbrakk>\<rbrakk> coin50_100 = \<lbrakk>\<rbrakk>"
+proof-
+  have consistent_medial: "consistent (medial \<lbrakk>\<rbrakk> (Guard coin50_100))"
+    apply (simp add: coin50_100_def consistent_def)
+    apply (rule_tac x="<I 1 := Num 50>" in exI)
+    by (simp add: consistent_empty_4)
+  show ?thesis
+    apply (simp add: posterior_def Let_def consistent_medial)
+    by (simp add: coin50_100_def)
+qed
+
+lemma posterior_coin100_100: "posterior \<lbrakk>\<rbrakk> coin100_100 = \<lbrakk>\<rbrakk>"
+proof-
+  have consistent_medial: "consistent (medial \<lbrakk>\<rbrakk> (Guard coin100_100))"
+    apply (simp add: coin100_100_def consistent_def)
+    apply (rule_tac x="<I 1 := Num 100>" in exI)
+    by (simp add: consistent_empty_4)
+  show ?thesis
+    apply (simp add: posterior_def Let_def consistent_medial)
+    by (simp add: coin100_100_def)
+qed
+
+lemma posterior_vend_coke: "posterior \<lbrakk>\<rbrakk> vend_coke = \<lbrakk>\<rbrakk>"
+proof-
+  have consistent_medial: "consistent (medial \<lbrakk>\<rbrakk> (Guard vend_coke))"
+    apply (simp add: vend_coke_def consistent_def)
+    apply (rule_tac x="<>" in exI)
+    by (simp add: consistent_empty_4)
+  show ?thesis
+    apply (simp add: posterior_def Let_def consistent_medial)
+    by (simp add: vend_coke_def)
+qed
+
+lemma posterior_vend_pepsi: "posterior \<lbrakk>\<rbrakk> vend_pepsi = \<lbrakk>\<rbrakk>"
+proof-
+  have consistent_medial: "consistent (medial \<lbrakk>\<rbrakk> (Guard vend_pepsi))"
+    apply (simp add: vend_pepsi_def consistent_def)
+    apply (rule_tac x="<>" in exI)
+    by (simp add: consistent_empty_4)
+  show ?thesis
+    apply (simp add: posterior_def Let_def consistent_medial)
+    by (simp add: vend_pepsi_def)
+qed
+
+lemma no_subsumption_coin50_50_coin50_100:  "\<not> subsumes \<lbrakk>\<rbrakk> coin50_50 coin50_100"
+proof-
+  have subsumption_violation: "(\<exists>i r. satisfies_context r \<lbrakk>\<rbrakk> \<and>
+           apply_guards (Guard coin50_100) (case_vname (\<lambda>n. input2state i 1 (I n)) (\<lambda>n. r (R n))) \<and>
+           apply_outputs (Outputs coin50_100) (case_vname (\<lambda>n. input2state i 1 (I n)) (\<lambda>n. r (R n))) \<noteq>
+           apply_outputs (Outputs coin50_50) (case_vname (\<lambda>n. input2state i 1 (I n)) (\<lambda>n. r (R n))))"
+    apply (simp add: coin50_50_def coin50_100_def)
+    apply standard
+     apply (rule_tac x="<>" in exI)
+     apply (simp add: satisfies_context_def datastate2context_def consistent_def)
+     apply (rule_tac x="<>" in exI)
+     apply clarify
+     defer
+    apply (rule_tac x="[Num 50]" in exI)
+    apply simp
+     apply (case_tac r)
+        apply simp
+       apply (case_tac x2)
+    by auto
+  show ?thesis
+    by (simp add: subsumes_def subsumption_violation)
+qed
+
+lemma no_subsumption_coin50_100_coin50_50: " \<not> subsumes \<lbrakk>\<rbrakk> coin50_100 coin50_50"
+proof-
+  have subsumption_violation: "(\<exists>i r. satisfies_context r \<lbrakk>\<rbrakk> \<and>
+           apply_guards (Guard coin50_50) (case_vname (\<lambda>n. input2state i 1 (I n)) (\<lambda>n. r (R n))) \<and>
+           apply_outputs (Outputs coin50_50) (case_vname (\<lambda>n. input2state i 1 (I n)) (\<lambda>n. r (R n))) \<noteq>
+           apply_outputs (Outputs coin50_100) (case_vname (\<lambda>n. input2state i 1 (I n)) (\<lambda>n. r (R n))))"
+        apply (simp add: coin50_50_def coin50_100_def)
+    apply standard
+     apply (rule_tac x="<>" in exI)
+     apply (simp add: satisfies_context_def datastate2context_def consistent_def)
+     apply (rule_tac x="<>" in exI)
+     apply clarify
+     defer
+    apply (rule_tac x="[Num 50]" in exI)
+    apply simp
+     apply (case_tac r)
+        apply simp
+       apply (case_tac x2)
+    by auto
+  show ?thesis
+    by (simp add: subsumes_def subsumption_violation)
+qed
+
+lemma no_subsumption_vend_coke_vend_pepsi: "\<not> subsumes \<lbrakk>\<rbrakk> vend_coke vend_pepsi"
+proof-
+  have subsumption_violation: "(\<exists>i r. satisfies_context r \<lbrakk>\<rbrakk> \<and>
+           apply_guards (Guard vend_pepsi) (case_vname (\<lambda>n. input2state i 1 (I n)) (\<lambda>n. r (R n))) \<and>
+           apply_outputs (Outputs vend_pepsi) (case_vname (\<lambda>n. input2state i 1 (I n)) (\<lambda>n. r (R n))) \<noteq>
+           apply_outputs (Outputs vend_coke) (case_vname (\<lambda>n. input2state i 1 (I n)) (\<lambda>n. r (R n))))"
+    apply (simp add: transitions)
+        apply (rule_tac x="<>" in exI)
+     apply (simp add: satisfies_context_def datastate2context_def consistent_def)
+     apply (rule_tac x="<>" in exI)
+     apply clarify
+     apply (case_tac r)
+        apply simp
+       apply (case_tac x2)
+    by auto
+  show ?thesis
+    by (simp add: subsumes_def subsumption_violation)
+qed
+
+lemma no_subsumption_vend_pepsi_vend_coke: "\<not> subsumes \<lbrakk>\<rbrakk> vend_pepsi vend_coke"
+proof-
+  have subsumption_violation: "(\<exists>i r. satisfies_context r \<lbrakk>\<rbrakk> \<and>
+           apply_guards (Guard vend_coke) (case_vname (\<lambda>n. input2state i 1 (I n)) (\<lambda>n. r (R n))) \<and>
+           apply_outputs (Outputs vend_coke) (case_vname (\<lambda>n. input2state i 1 (I n)) (\<lambda>n. r (R n))) \<noteq>
+           apply_outputs (Outputs vend_pepsi) (case_vname (\<lambda>n. input2state i 1 (I n)) (\<lambda>n. r (R n))))"
+    apply (simp add: transitions)
+        apply (rule_tac x="<>" in exI)
+     apply (simp add: satisfies_context_def datastate2context_def consistent_def)
+     apply (rule_tac x="<>" in exI)
+     apply clarify
+     apply (case_tac r)
+        apply simp
+       apply (case_tac x2)
+    by auto
+  show ?thesis
+    by (simp add: subsumes_def subsumption_violation)
+qed
+
+lemma step_pta_selectCoke: "step (tm pta) 0 Map.empty ''select'' [Str ''coke''] = Some (selectCoke, 1, [], <>)"
+proof-
+  have possible_steps: "possible_steps (tm pta) 0 Map.empty ''select'' [Str ''coke''] = {|(1, selectCoke)|}"
+    apply (simp add: possible_steps_def ffilter_def fimage_def fset_both_sides Abs_fset_inverse)
+    apply (simp add: tm_def pta_def Set.filter_def)
+    apply safe
+                      apply (simp_all add: transitions)
+    by force
+  show ?thesis
+    apply (simp add: step_def possible_steps)
+    by (simp add: selectCoke_def)
+qed
+
+lemma step_merged_2_9_selectCoke: "step (tm merged_2_9) 0 Map.empty ''select'' [Str ''coke''] = Some (selectCoke, 1, [], <>)"
+proof-
+  have possible_steps: "possible_steps (tm merged_2_9) 0 Map.empty ''select'' [Str ''coke''] = {|(1, selectCoke)|}"
+    apply (simp add: possible_steps_fst)
+    apply (simp add: tm_def merged_2_9_def Set.filter_def)
+    apply safe
+      apply (simp_all add: transitions)
+    by force
+  show ?thesis
+    apply (simp add: step_def possible_steps)
+    by (simp add: selectCoke_def)
+qed
+
+definition merged_1_7 :: iEFSM where
+  "merged_1_7 = {|(0, (0, 1), selectCoke), (2, (1, 2), coin50_50), (4, (2, 3), coin50_100),  (5, (3, 4), vend_coke), 
+                                                                   (3, (1, 5), coin100_100), (6, (5, 6), vend_coke),
+                 (1, (0, 1), selectPepsi), (7, (1, 8), coin50_50), (8, (8, 9), coin50_100),  (9, (9, 10), vend_pepsi)|}"
+
+lemma merge_states_1_7: "merge_states 1 7 pta = merged_1_7"
+  by (simp add: merge_states_def pta_def merge_states_aux_def merged_1_7_def)
+
+definition merged_2_8 :: iEFSM where
+  "merged_2_8 = {|(0, (0, 1), selectCoke),  (2, (1, 2), coin50_50),  (4, (2, 3), coin50_100),  (5, (3, 4), vend_coke),
+                                                                      (3, (1, 5), coin100_100), (6, (5, 6), vend_coke),
+                   (1, (0, 1), selectPepsi), (7, (1, 2), coin50_50),  (8, (2, 9), coin50_100),  (9, (9, 10), vend_pepsi)|}"
+
+lemma merge_states_2_8: "merge_states 2 8 merged_1_7 = merged_2_8"
+  by (simp add: merge_states_def merge_states_aux_def merged_1_7_def merged_2_8_def)
+
+lemma no_choice_coin50_50_coin100_100: "\<not>choice coin50_50 coin100_100"
+  by (simp add: choice_def transitions)
+
+definition merge_2_8_no_nondet :: iEFSM where
+  "merge_2_8_no_nondet = {|(0, (0, 1), selectCoke), (2, (1, 2), coin50_50), (4, (2, 3), coin50_100), (5, (3, 4), vend_coke), (3, (1, 5), coin100_100),
+      (6, (5, 6), vend_coke), (1, (0, 1), selectPepsi), (7, (1, 2), coin50_50), (8, (2, 9), coin50_100), (9, (9, 10), vend_pepsi)|}"
+
+definition selectGeneral :: transition where
+  "selectGeneral = \<lparr>Label = ''select'', Arity = 1, Guard = [], Outputs = [], Updates = [(R 1, V (I 1))]\<rparr>"
+
+definition vend_general :: transition where
+  "vend_general = \<lparr>Label = ''vend'', Arity = 0, Guard = [], Outputs = [V (R 1)], Updates = []\<rparr>"
+
+definition merged_4_10 :: iEFSM where
+  "merged_4_10 = {|(0, (0, 1), selectCoke), (2, (1, 2), coin50_50), (4, (2, 3), coin50_100), (5, (3, 4), vend_coke) ,
+                   (1, (0, 1), selectPepsi),                                                 (9, (3, 4), vend_pepsi), 
+                                            (3, (1, 5), coin100_100), (6, (5, 6), vend_coke)|}"
+
+definition merged_vends :: iEFSM where
+  "merged_vends = {|(0, (0, 1), selectGeneral), (2, (1, 2), coin50_50), (4, (2, 3), coin50_100), (5, (3, 4), vend_general) ,
+                                            (3, (1, 5), coin100_100), (6, (5, 6), vend_general)|}"
+
+definition coinGeneral :: transition where
+  "coinGeneral = \<lparr>Label = ''coin'', Arity = 1, Guard = [], Outputs = [Plus (V (I 1)) (V (R 2))], Updates = [(R 2, Plus (V (I 1)) (V (R 2)))]\<rparr>"
+
+lemma no_choice_coin100_100_coin50_50: "\<not>choice coin100_100 coin50_50"
+  by (simp add: choice_def transitions)
+
+lemma no_choice_coin100_100_coin50_100: "\<not>choice coin100_100 coin50_100"
+  by (simp add: choice_def transitions)
+
+lemma no_choice_selectCoke_selectPepsi: "\<not>choice selectCoke selectPepsi"
+  by (simp add: choice_def transitions)
+
+lemma choice_coin50_100_coin50_50: "choice coin50_100 coin50_50"
+  apply (simp add: choice_def transitions)
+  by auto
+
+lemma choice_coin50_50_coin50_50: "choice coin50_50 coin50_50"
+  apply (simp add: choice_def transitions)
+  by auto
+
+lemma choice_coin50_100_coin50_100: "choice coin50_100 coin50_100"
+  apply (simp add: choice_def transitions)
+  by auto
+
+lemma choice_vend_coke_vend_pepsi: "choice vend_coke vend_pepsi"
+  by (simp add: choice_def transitions)
+
+lemma no_coice_vend_general_coin100_100:  "\<not>choice vend_general coin100_100"
+  by (simp add: choice_def transitions vend_general_def)
+
+lemma no_choice_coinGeneral_vend_general: "\<not>choice coinGeneral vend_general"
+  by (simp add: choice_def coinGeneral_def vend_general_def)
+
+lemma choice_coinGeneral_coin100_100: "choice coinGeneral coin100_100"
+  apply (simp add: transitions coinGeneral_def choice_def)
+  by auto
+
+lemma no_coice_coin100_100_vend_general: "\<not>choice coin100_100 vend_general"
+  by (simp add: choice_def transitions vend_general_def)
+
+lemma choice_coin100_100_coinGeneral: "choice coin100_100 coinGeneral"
+  apply (simp add: transitions coinGeneral_def choice_def)
+  by auto
+
+lemma choice_vend_general_vend_general: "choice vend_general vend_general"
+  by (simp add: choice_def vend_general_def)
+
+lemmas choices = choice_vend_general_vend_general choice_coin100_100_coinGeneral  no_coice_coin100_100_vend_general choice_coinGeneral_coin100_100 no_choice_coinGeneral_vend_general no_coice_vend_general_coin100_100 choice_vend_coke_vend_pepsi choice_coin50_100_coin50_100 choice_coin50_50_coin50_50 choice_coin50_100_coin50_50 no_choice_selectCoke_selectPepsi no_choice_coin100_100_coin50_100 no_choice_coin100_100_coin50_50 no_choice_coin50_50_coin100_100 choice_symmetry
+
+lemma coin50_50_lt_coin50_100: "coin50_50 < coin50_100"
+  by (simp add: transitions less_transition_ext_def less_aexp_def)
+
+lemma vend_coke_lt_vend_pepsi: "vend_coke < vend_pepsi"
+  by (simp add: transitions less_transition_ext_def less_aexp_def)
+
+lemmas orders = vend_coke_lt_vend_pepsi coin50_50_lt_coin50_100
 
 lemma merge_states_1_8: "merge_states 1 8 pta = merged_1_8"
   apply (simp add: merge_states_def merge_states_aux_def pta_def merged_1_8_def)
@@ -69,21 +874,6 @@ proof-
     by (simp_all add: choices)
 qed
 
-definition selectGeneral :: transition where
-  "selectGeneral = \<lparr>Label = ''select'', Arity = 1, Guard = [], Outputs = [], Updates = [(R 1, V (I 1))]\<rparr>"
-
-definition vend_general :: transition where
-  "vend_general = \<lparr>Label = ''vend'', Arity = 0, Guard = [], Outputs = [V (R 1)], Updates = []\<rparr>"
-
-definition merged_4_10 :: iEFSM where
-  "merged_4_10 = {|(0, (0, 1), selectCoke), (2, (1, 2), coin50_50), (4, (2, 3), coin50_100), (5, (3, 4), vend_coke) ,
-                   (1, (0, 1), selectPepsi),                                                 (9, (3, 4), vend_pepsi), 
-                                            (3, (1, 5), coin100_100), (6, (5, 6), vend_coke)|}"
-
-definition merged_vends :: iEFSM where
-  "merged_vends = {|(0, (0, 1), selectGeneral), (2, (1, 2), coin50_50), (4, (2, 3), coin50_100), (5, (3, 4), vend_general) ,
-                                            (3, (1, 5), coin100_100), (6, (5, 6), vend_general)|}"
-
 definition generator :: generator_function where
   "generator oldEFSM t1FromOld t1 t2FromOld t2 = (if (oldEFSM, t1FromOld, t1, t2FromOld, t2) = (pta, 1, coin50_50, 8, coin50_100) then None
                                                   else None)"
@@ -100,8 +890,6 @@ definition H_merged_1_2 :: "nat \<Rightarrow> nat" where
 definition merged_1_3 :: iEFSM where
   "merged_1_3 = {|(0, (0, 1), selectGeneral), (2, (1, 1), coin50_50), (4, (1, 1), coin50_100), (5, (1, 4), vend_general),
                                               (3, (1, 5), coin100_100), (6, (5, 6), vend_general)|}"
-definition coinGeneral :: transition where
-  "coinGeneral = \<lparr>Label = ''coin'', Arity = 1, Guard = [], Outputs = [Plus (V (I 1)) (V (R 2))], Updates = [(R 2, Plus (V (I 1)) (V (R 2)))]\<rparr>"
 
 definition selectGeneral_2 :: transition where
   "selectGeneral_2 = \<lparr>Label = ''select'', Arity = 1, Guard = [], Outputs = [], Updates = [(R 1, V (I 1)), (R 2, (L (Num 0)))]\<rparr>"
@@ -1936,16 +2724,6 @@ lemma nondeterministic_simulates_merged_1_3_coin_merged_vends: "nondeterministic
   apply (simp add: nondeterministic_simulates_def)
   by (simp add: nondeterministic_simulates_trace_merged_1_3_coin_merged_vends_0_0)
 
-lemma no_coice_vend_general_coin100_100:  "\<not>choice vend_general coin100_100"
-  by (simp add: choice_def transitions vend_general_def)
-
-lemma no_choice_coinGeneral_vend_general: "\<not>choice coinGeneral vend_general"
-  by (simp add: choice_def coinGeneral_def vend_general_def)
-
-lemma choice_coinGeneral_coin100_100: "choice coinGeneral coin100_100"
-  apply (simp add: transitions coinGeneral_def choice_def)
-  by auto
-
 lemma nondeterministic_pairs_merged_1_3_coin: "nondeterministic_pairs merged_1_3_coin = {|(1, (1, 5), (coinGeneral, 2), coin100_100, 3)|}"
 proof-
   have minus_1: "{|(1, coinGeneral, 2), (4, vend_general, 5), (5, coin100_100, 3)|} |-| {|(4, vend_general, 5)|} = {|(1, coinGeneral, 2), (5, coin100_100, 3)|}"
@@ -1963,7 +2741,7 @@ proof-
     apply (simp add: outgoing_transitions_def fimage_def state_nondeterminism_1)
     apply (simp add: ffilter_def Set.filter_def fset_both_sides Abs_fset_inverse)
     apply safe
-                 apply (simp_all add: choices no_coice_vend_general_coin100_100 no_choice_coinGeneral_vend_general choice_coinGeneral_coin100_100)
+                 apply (simp_all add: choices)
     by (simp add: coinGeneral_def transitions less_transition_ext_def)
 qed
 
@@ -1972,9 +2750,6 @@ definition merged_4_6 :: iEFSM where
 
 definition final :: iEFSM where
   "final = {|(0, (0, 1), selectGeneral_2), (2, (1, 1), coinGeneral), (5, (1, 4), vend_general)|}"
-
-lemma choice_vend_general_vend_general: "choice vend_general vend_general"
-  by (simp add: choice_def vend_general_def)
 
 lemma directly_subsumes_vend_general_self: "directly_subsumes (tm merged_vends) (tm merged_4_6) 5 vend_general vend_general"
 proof-
@@ -2001,348 +2776,9 @@ proof-
     apply (simp add: outgoing_transitions_def fimage_def state_nondeterminim_1)
     apply (simp add: ffilter_def fset_both_sides Abs_fset_inverse Set.filter_def)
     apply safe
-    by (simp_all add: choices no_choice_coinGeneral_vend_general choice_vend_general_vend_general)
+    by (simp_all add: choices)
 qed
 
-lemma no_route_from_4_to_1: "\<not>gets_us_to 1 (tm merged_vends) 4 r' list"
-proof(induct list)
-  case Nil
-  then show ?case
-    by (simp add: no_further_steps)
-next
-  have possible_steps_merged_vends_4: "\<forall>r l i. possible_steps (tm merged_vends) 4 r l i = {||}"
-    apply (simp add: possible_steps_fst)
-    by (simp add: merged_vends_def Set.filter_def tm_def)
-  case (Cons a list)
-  then show ?case
-    apply safe
-    apply (rule gets_us_to.cases)
-       apply simp
-      apply simp
-     apply clarify
-    apply (simp add: step_def possible_steps_merged_vends_4)
-    apply clarify
-    by simp
-qed
-
-lemma no_route_from_3_to_1: "\<not>gets_us_to 1 (tm merged_vends) 3 r'a list"
-proof(induct list)
-  case Nil
-  then show ?case
-    by (simp add: no_further_steps)
-next
-  have possible_steps_not_vend: "\<And>aa ba r.
-       aa = ''vend'' \<longrightarrow> ba \<noteq> [] \<Longrightarrow>
-       possible_steps (tm merged_vends) 3 r aa ba = {||}"
-    apply (simp add: possible_steps_fst)
-    apply (simp add: tm_def merged_vends_def Set.filter_def)
-    apply (simp add: vend_general_def)
-    by auto
-  have singleton_vend: "\<forall>r a aa b. fis_singleton (possible_steps (tm merged_vends) 3 r aa b) \<longrightarrow> aa = ''vend'' \<and> b = []"
-    apply clarify
-    apply (case_tac "aa = ''vend'' \<and> b = []")
-     apply simp
-    by (simp add: possible_steps_not_vend)
-  case (Cons a list)
-  then show ?case
-    apply clarify
-    apply (case_tac "a = (''vend'', [])")
-     apply (rule gets_us_to.cases)
-        apply simp
-       apply simp
-      apply clarify
-      apply (simp add: step_def possible_steps_vend vend_general_def)
-      apply clarify
-      apply (simp add: no_route_from_4_to_1)
-     apply clarify
-     apply simp
-
-    apply (rule gets_us_to.cases)
-        apply simp
-       apply simp
-     apply clarify
-     apply (simp add: step_def)
-    apply (case_tac "fis_singleton (possible_steps (tm merged_vends) 3 r'a aa b)")
-      apply (case_tac "fthe_elem (possible_steps (tm merged_vends) 3 r'a aa b)")
-      apply (simp add: singleton_vend)
-     apply (simp add: singleton_vend)
-    apply clarify
-    by simp
-qed
-
-lemma no_route_from_2_to_1: "\<not>gets_us_to 1 (tm merged_vends) 2 r' list"
-proof(induct list)
-  case Nil
-  then show ?case
-    by (simp add: no_further_steps)
-next
-  have possible_steps_not_coin: "\<And>aa ba r.
-       aa = ''coin'' \<longrightarrow> ba \<noteq> [Num 50] \<Longrightarrow>
-       possible_steps (tm merged_vends) 2 r aa ba = {||}"
-    apply (simp add: possible_steps_fst)
-    apply (simp add: tm_def merged_vends_def Set.filter_def)
-    apply (simp add: coin50_100_def hd_input2state)
-    by (metis One_nat_def length_0_conv length_Suc_conv list.sel(1))
-  have singleton_coin: "\<forall>r' aa b. fis_singleton (possible_steps (tm merged_vends) 2 r' aa b) \<longrightarrow> aa = ''coin'' \<and> b = [Num 50]"
-    apply clarify
-    apply (case_tac "aa = ''coin'' \<and> b = [Num 50]")
-     apply simp
-    by (simp add: possible_steps_not_coin)
-  case (Cons a list)
-  then show ?case
-    apply clarify
-    apply (case_tac "a = (''coin'', [Num 50])")
-     apply (rule gets_us_to.cases)
-        apply simp
-       apply simp
-      apply clarify
-      apply (simp add: step_def possible_steps_merged_vends_coin50_2 no_route_from_3_to_1)
-     apply clarify
-     apply simp
-
-     apply (rule gets_us_to.cases)
-        apply simp
-       apply simp
-     apply clarify
-     apply simp
-     apply (simp add: step_def)
-     apply (case_tac "fis_singleton (possible_steps (tm merged_vends) 2 r' aa b)")
-      apply simp
-      apply (case_tac "fthe_elem (possible_steps (tm merged_vends) 2 r' aa b)")
-      apply simp
-      apply clarify
-      apply (simp add: singleton_coin)
-     apply simp
-    by simp
-qed
-
-lemma no_route_from_6_to_1: "\<not>gets_us_to 1 (tm merged_vends) 6 r'a list"
-proof(induct list)
-  case Nil
-  then show ?case
-    by (simp add: no_further_steps)
-next
-  have stop: "\<forall>r aaa ba. possible_steps (tm merged_vends) 6 r aaa ba = {||}"
-    apply (simp add: possible_steps_fst)
-    by (simp add: tm_def merged_vends_def Set.filter_def)
-  case (Cons a list)
-  then show ?case
-    apply safe
-    apply (rule gets_us_to.cases)
-       apply simp
-      apply simp
-     apply clarify
-     apply (simp add: step_def stop)
-    apply clarify
-    by simp
-qed
-
-lemma no_route_from_5_to_1: "\<not>gets_us_to 1 (tm merged_vends) 5 r' list"
-proof(induct list)
-  case Nil
-  then show ?case
-    by (simp add: no_further_steps)
-next
-  have possible_steps_vend: "\<forall>r. possible_steps (tm merged_vends) 5 r ''vend'' [] = {|(6, vend_general)|}"
-    apply (simp add: possible_steps_fst)
-    apply (simp add: tm_def merged_vends_def Set.filter_def)
-    apply (simp add: transitions vend_general_def)
-    by force
-  have stop_2: "\<And>aa ba r.
-       aa = ''vend'' \<longrightarrow> ba \<noteq> [] \<Longrightarrow>
-       possible_steps (tm merged_vends) 5 r aa ba = {||}"
-    apply (simp add: possible_steps_fst)
-    apply (simp add: tm_def merged_vends_def Set.filter_def vend_general_def)
-    by auto
-  case (Cons a list)
-  then show ?case
-apply clarify
-    apply (case_tac "a = (''vend'', [])")
-     apply (rule gets_us_to.cases)
-        apply simp
-       apply simp
-      apply clarify
-      apply (simp add: step_def possible_steps_vend vend_general_def)
-      apply clarify
-      apply (simp add: no_route_from_6_to_1)
-     apply clarify
-     apply simp
-
-    apply (rule gets_us_to.cases)
-        apply simp
-       apply simp
-     apply clarify
-     apply (simp add: step_def)
-     apply (case_tac "fis_singleton (possible_steps (tm merged_vends) 5 r' aa b)")
-      apply simp
-      apply (case_tac "a = (''vend'', [])")
-       apply simp
-      apply (simp add: stop_2)
-     apply simp
-    apply clarify
-    by simp
-qed
-
-lemma not_go_to_1_aux: "gets_us_to 1 (tm merged_vends) 1 r ((aa, ba) # list) \<Longrightarrow> \<not>accepts (tm merged_vends) 1 r ((aa, ba) # list)"
-proof-
-  assume premise: "gets_us_to 1 (tm merged_vends) 1 r ((aa, ba) # list)"
-  have stop: "\<And>aa ba r.
-       aa = ''coin'' \<longrightarrow> ba \<noteq> [Num 50] \<Longrightarrow>
-       aa = ''coin'' \<longrightarrow> ba \<noteq> [Num 100] \<Longrightarrow>
-       possible_steps (tm merged_vends) 1 r aa ba = {||}"
-    apply (simp add: possible_steps_fst)
-    apply (simp add: tm_def merged_vends_def Set.filter_def)
-    apply (simp add: coin50_50_def coin100_100_def)
-    apply clarify
-    apply simp
-    apply (case_tac "b=2")
-     apply (simp add: hd_input2state)
-     apply (metis One_nat_def length_0_conv length_Suc_conv list.sel(1))
-    apply (case_tac "b=5")
-     apply (simp add: hd_input2state)
-     apply (metis One_nat_def length_0_conv length_Suc_conv list.sel(1))
-    by simp
-  show ?thesis
-    using premise
-    apply (case_tac "aa = ''coin'' \<and> ba = [Num 50]")
-     apply simp
-     apply (rule gets_us_to.cases)
-        apply simp
-       apply simp
-      apply clarify
-      apply (simp add: step_def possible_steps_merged_vends_coin50_1 coin50_50_def no_route_from_2_to_1)
-     apply clarify
-     apply simp
-     apply (simp add: step_def possible_steps_merged_vends_coin50_1)
-  
-    apply (case_tac "aa = ''coin'' \<and> ba = [Num 100]")
-     apply simp
-     apply (rule gets_us_to.cases)
-        apply simp
-       apply simp
-      apply clarify
-      apply (simp add: step_def possible_steps_merged_vends_coin100 coin100_100_def no_route_from_5_to_1)
-     apply clarify
-     apply simp
-     apply (simp add: step_def possible_steps_merged_vends_coin100)
-    apply clarify
-    apply (rule accepts.cases)
-      apply simp
-     apply simp
-    apply clarify
-    by (simp add: step_def stop)
-qed
-
-lemma not_go_to_1: "length b = 1 \<Longrightarrow>
-       accepts_trace (tm merged_vends) ((''select'', b) # (aa, ba) # list) \<Longrightarrow>
-       \<not>gets_us_to 1 (tm merged_vends) 0 Map.empty ((''select'', b) # (aa, ba) # list)"
-proof-
-  assume premise1: "length b = 1"
-  assume premise2: "accepts_trace (tm merged_vends) ((''select'', b) # (aa, ba) # list)"
-  have possible_steps_select: "\<forall>d. length d = 1 \<longrightarrow> possible_steps (tm merged_vends) 0 Map.empty ''select'' d = {|(1, selectGeneral)|}"
-    apply (simp add: possible_steps_fst)
-    apply (simp add: tm_def merged_vends_def Set.filter_def)
-    apply safe
-              apply (simp_all add: transitions selectGeneral_def)
-    by force
-  show ?thesis
-    apply safe
-    apply (rule gets_us_to.cases)
-       apply simp
-      apply simp
-     apply clarify
-    using premise1
-     apply (simp add: step_def possible_steps_select)
-     apply clarify
-    using premise2
-     apply (simp add: accepts_trace_def)
-     apply (rule accepts.cases)
-       apply simp
-      apply simp
-     apply clarify
-     apply (simp add: step_def possible_steps_select selectGeneral_def)
-     apply clarify
-     apply simp
-     apply (simp add: not_go_to_1_aux)
-    apply clarify
-    by (simp add: step_def)
-qed
-
-lemma invalid_input: "aa = ''select'' \<longrightarrow> length b \<noteq> 1 \<Longrightarrow>
-       \<not>accepts_trace (tm merged_vends) ((aa, b) # p)"
-proof-
-  assume premise: "aa = ''select'' \<longrightarrow> length b \<noteq> 1"
-  have invalid_possible_steps: "possible_steps (tm merged_vends) 0 Map.empty aa b = {||}"
-    using premise
-    apply (simp add: possible_steps_fst)
-    apply (simp add: Set.filter_def tm_def merged_vends_def)
-    apply safe
-    by (simp_all add: selectGeneral_def)
-  show ?thesis
-    apply clarify
-    apply (simp add: accepts_trace_def)
-    apply (rule accepts.cases)
-      apply simp
-     apply simp
-    apply (simp add: step_def)
-    apply clarify
-    by (simp add: invalid_possible_steps)
-qed
-
-lemma merged_1_5_anterior: " accepts_trace (tm merged_vends) p \<longrightarrow>
-        gets_us_to 1 (tm merged_vends) 0 Map.empty p \<longrightarrow>
-        anterior_context (tm merged_1_5) p = \<lbrakk>V (R 1) \<mapsto> Bc True, V (R 2) \<mapsto> Eq (Num 0)\<rbrakk>"
-proof (induct p)
-  case Nil
-  then show ?case
-    by (simp add: no_further_steps)
-next
-  have possible_steps_select: "\<forall>b. length b = 1 \<longrightarrow> possible_steps (tm merged_1_5) 0 Map.empty ''select'' b = {|(1, selectGeneral_2)|}"
-    apply (simp add: possible_steps_fst)
-    apply (simp add: tm_def merged_1_5_def Set.filter_def)
-    apply safe
-          apply (simp_all add: selectGeneral_2_def)
-    by force
-  have posterior_empty_selectGeneral_2: "posterior \<lbrakk>\<rbrakk> selectGeneral_2 = \<lbrakk>V (R 1) \<mapsto> Bc True, V (R 2) \<mapsto> Eq (Num 0)\<rbrakk>"
-    apply (rule ext)
-    by (simp add: posterior_def selectGeneral_2_def remove_input_constraints_def)
-  case (Cons a p)
-  then show ?case
-    apply (case_tac a)
-    apply (case_tac "aa = ''select'' \<and> length b = 1")
-     apply (simp add: anterior_context_def step_def possible_steps_select posterior_empty_selectGeneral_2)
-     apply (case_tac p)
-      apply simp
-      apply clarify
-      apply (rule ext)
-      apply simp
-     apply (case_tac p)
-      apply simp
-     apply simp
-     apply clarify
-     apply simp
-     apply (simp add: not_go_to_1)
-    apply simp
-    by (simp add: invalid_input)
-qed
-
-lemma satisfies_context: "satisfies_context r \<lbrakk>V (R 1) \<mapsto> cexp.Bc True, V (R 2) \<mapsto> cexp.Eq (Num 0)\<rbrakk> \<Longrightarrow> r (R 2) = Some (Num 0)"
-proof-
-  assume premise: "satisfies_context r \<lbrakk>V (R 1) \<mapsto> cexp.Bc True, V (R 2) \<mapsto> cexp.Eq (Num 0)\<rbrakk>"
-  have contra: "\<not>r (R 2) = Some (Num 0)  \<Longrightarrow> \<not>satisfies_context r \<lbrakk>V (R 1) \<mapsto> cexp.Bc True, V (R 2) \<mapsto> cexp.Eq (Num 0)\<rbrakk>"
-    apply (simp add: satisfies_context_def datastate2context_def consistent_def)
-    apply clarify
-    apply (rule_tac x="V (R 2)" in exI)
-    apply simp
-    apply (case_tac "r (R 2)")
-     apply simp
-    by simp
-  show ?thesis
-    using premise contra
-    by auto
-qed
-
-(*This isn't true because coin100_100 doesn't update r2*)
 lemma no_direct_subsumption_coinGeneral_coin100_100:  "\<not>directly_subsumes (tm merged_vends) (tm merged_1_5) 1 coinGeneral coin100_100"
 proof-
   have possible_steps: "\<forall>d. possible_steps (tm merged_vends) 0 Map.empty ''select'' [d] = {|(1, selectGeneral)|}"
